mlanguage: remove concurrency bits

theories/mlanguage/mlanguage.v
@@ -2,8 +2,6 @@ From stdpp Require Import relations strings gmap.
 From iris.algebra Require Import ofe.
 From iris.prelude Require Import options.
 
-Definition thread_id := nat.
-
 Section mlanguage_mixin.
   Context {expr val func ectx public_state private_state state : Type}.
 
@@ -20,16 +18,11 @@ Section mlanguage_mixin.
   Context (fill : ectx → expr → expr).
   Context (split_state : state → public_state → private_state → Prop).
 
-  (** Parallel substitution, to define [log_rel] in a language-independent
-      way. *)
-  (* Context (subst_map : gmap string val → expr → expr). *)
-  (* Context (free_vars : expr → gset string). *)
-
   (** A program is a map from function names to function bodies. *)
   Local Notation mixin_prog := (gmap string func).
 
   Context (apply_func : func → list val → option expr).
-  Context (head_step : mixin_prog → expr → state → expr → state → list expr → Prop).
+  Context (head_step : mixin_prog → expr → state → expr → state → Prop).
 
   Record MlanguageMixin := {
     (** Expression classification *)
@@ -38,12 +31,12 @@ Section mlanguage_mixin.
 
     (** Reduction behavior of the special classes of expressions *)
     (** mixin_val_head_step is not an iff because the backward direction is trivial *)
-    mixin_val_head_step p v σ1 e2 σ2 efs :
-      head_step p (of_class (ExprVal v)) σ1 e2 σ2 efs → False;
-    mixin_call_head_step p f vs σ1 e2 σ2 efs :
-      head_step p (of_class (ExprCall f vs)) σ1 e2 σ2 efs ↔
+    mixin_val_head_step p v σ1 e2 σ2 :
+      head_step p (of_class (ExprVal v)) σ1 e2 σ2 → False;
+    mixin_call_head_step p f vs σ1 e2 σ2 :
+      head_step p (of_class (ExprCall f vs)) σ1 e2 σ2 ↔
       ∃ (fn : func),
-        p !! f = Some fn ∧ Some e2 = apply_func fn vs ∧ σ2 = σ1 ∧ efs = [];
+        p !! f = Some fn ∧ Some e2 = apply_func fn vs ∧ σ2 = σ1;
 
     (** Evaluation contexts *)
     mixin_fill_empty e : fill empty_ectx e = e;
@@ -72,10 +65,10 @@ Section mlanguage_mixin.
 
         This implies there can be only one head redex, see
         [head_redex_unique]. *)
-    mixin_step_by_val p K' K_redex e1' e1_redex σ1 e2 σ2 efs :
+    mixin_step_by_val p K' K_redex e1' e1_redex σ1 e2 σ2 :
       fill K' e1' = fill K_redex e1_redex →
       match to_class e1' with Some (ExprVal _) => False | _ => True end →
-      head_step p e1_redex σ1 e2 σ2 efs →
+      head_step p e1_redex σ1 e2 σ2 →
       ∃ K'', K_redex = comp_ectx K' K'';
 
     (** If [fill K e] takes a head step, then either [e] is a value or [K] is
@@ -83,8 +76,8 @@ Section mlanguage_mixin.
         wrapping it in a context does not add new head redex positions. *)
     (* FIXME: This is the exact same conclusion as [mixin_fill_class]... is
        there some pattern or reduncancy here? *)
-    mixin_head_ctx_step_val p K e σ1 e2 σ2 efs :
-      head_step p (fill K e) σ1 e2 σ2 efs → K = empty_ectx ∨ ∃ v, to_class e = Some (ExprVal v);
+    mixin_head_ctx_step_val p K e σ1 e2 σ2 :
+      head_step p (fill K e) σ1 e2 σ2 → K = empty_ectx ∨ ∃ v, to_class e = Some (ExprVal v);
   }.
 End mlanguage_mixin.
 
@@ -105,7 +98,7 @@ Structure mlanguage {val : Type} {public_state : Type} := Mlanguage {
   fill : ectx → expr → expr;
   split_state : state → public_state → private_state → Prop;
   apply_func : func → list val → option expr;
-  head_step : mixin_prog func → expr → state → expr → state → list expr → Prop;
+  head_step : mixin_prog func → expr → state → expr → state → Prop;
 
   mlanguage_mixin :
     MlanguageMixin (val:=val) of_class to_class empty_ectx comp_ectx fill
@@ -124,7 +117,7 @@ Arguments comp_ectx {_ _ _} _ _.
 Arguments fill {_ _ _} _ _.
 Arguments split_state {_ _ _} _ _.
 Arguments apply_func {_ _ _}.
-Arguments head_step {_ _ _} _ _ _ _ _ _.
+Arguments head_step {_ _ _} _ _ _ _ _.
 
 Definition expr_class {val state} (Λ : mlanguage val state) := mixin_expr_class val.
 (* A [Definition] throws off Coq's "old" ("tactic") unification engine *)
@@ -155,7 +148,6 @@ Section mlanguage.
   Implicit Types c : expr_class Λ.
   Implicit Types K : ectx Λ.
   Implicit Types p : prog Λ.
-  Implicit Types efs : list (expr Λ).
 
   Lemma to_of_class c : to_class (of_class Λ c) = Some c.
   Proof. apply mlanguage_mixin. Qed.
@@ -171,12 +163,12 @@ Section mlanguage.
   Lemma is_call_is_class e : is_Some (to_call e) → is_Some (to_class e).
   Proof. rewrite /to_call /is_Some. destruct (to_class e) as [[|]|]; naive_solver. Qed.
 
-  Lemma val_head_step p v σ1 e2 σ2 efs :
-    head_step p (of_class Λ (ExprVal v)) σ1 e2 σ2 efs → False.
+  Lemma val_head_step p v σ1 e2 σ2 :
+    head_step p (of_class Λ (ExprVal v)) σ1 e2 σ2 → False.
   Proof. apply mlanguage_mixin. Qed.
-  Lemma call_head_step p f vs σ1 e2 σ2 efs :
-    head_step p (of_class Λ (ExprCall f vs)) σ1 e2 σ2 efs ↔
-    ∃ fn, p !! f = Some fn ∧ Some e2 = apply_func fn vs ∧ σ2 = σ1 ∧ efs = nil.
+  Lemma call_head_step p f vs σ1 e2 σ2 :
+    head_step p (of_class Λ (ExprCall f vs)) σ1 e2 σ2 ↔
+    ∃ fn, p !! f = Some fn ∧ Some e2 = apply_func fn vs ∧ σ2 = σ1.
   Proof. apply mlanguage_mixin. Qed.
 
   Lemma fill_empty e : fill empty_ectx e = e.
@@ -188,14 +180,14 @@ Section mlanguage.
   Lemma fill_class' K e :
     is_Some (to_class (fill K e)) → K = empty_ectx ∨ ∃ v, to_class e = Some (ExprVal v).
   Proof. apply mlanguage_mixin. Qed.
-  Lemma step_by_val' p K' K_redex e1' e1_redex σ1 e2 σ2 efs :
+  Lemma step_by_val' p K' K_redex e1' e1_redex σ1 e2 σ2 :
       fill K' e1' = fill K_redex e1_redex →
       match to_class e1' with Some (ExprVal _) => False | _ => True end →
-      head_step p e1_redex σ1 e2 σ2 efs →
+      head_step p e1_redex σ1 e2 σ2 →
       ∃ K'', K_redex = comp_ectx K' K''.
   Proof. apply mlanguage_mixin. Qed.
-  Lemma head_ctx_step_val' p K e σ1 e2 σ2 efs :
-    head_step p (fill K e) σ1 e2 σ2 efs → K = empty_ectx ∨ ∃ v, to_class e = Some (ExprVal v).
+  Lemma head_ctx_step_val' p K e σ1 e2 σ2 :
+    head_step p (fill K e) σ1 e2 σ2 → K = empty_ectx ∨ ∃ v, to_class e = Some (ExprVal v).
   Proof. apply mlanguage_mixin. Qed.
   Lemma fill_class K e :
     is_Some (to_class (fill K e)) → K = empty_ectx ∨ is_Some (to_val e).
@@ -203,37 +195,37 @@ Section mlanguage.
     intros [?|[v Hv]]%fill_class'; first by left. right.
     rewrite /to_val Hv. eauto.
   Qed.
-  Lemma step_by_val p K' K_redex e1' e1_redex σ1 e2 σ2 efs :
+  Lemma step_by_val p K' K_redex e1' e1_redex σ1 e2 σ2 :
       fill K' e1' = fill K_redex e1_redex →
       to_val e1' = None →
-      head_step p e1_redex σ1 e2 σ2 efs →
+      head_step p e1_redex σ1 e2 σ2 →
       ∃ K'', K_redex = comp_ectx K' K''.
   Proof.
     rewrite /to_val => ? He1'. eapply step_by_val'; first done.
     destruct (to_class e1') as [[]|]; done.
   Qed.
-  Lemma head_ctx_step_val p K e σ1 e2 σ2 efs :
-    head_step p (fill K e) σ1 e2 σ2 efs → K = empty_ectx ∨ is_Some (to_val e).
+  Lemma head_ctx_step_val p K e σ1 e2 σ2 :
+    head_step p (fill K e) σ1 e2 σ2 → K = empty_ectx ∨ is_Some (to_val e).
   Proof.
     intros [?|[v Hv]]%head_ctx_step_val'; first by left. right.
     rewrite /to_val Hv. eauto.
   Qed.
-  Lemma call_head_step_inv p f vs σ1 e2 σ2 efs :
-    head_step p (of_class Λ (ExprCall f vs)) σ1 e2 σ2 efs →
-    ∃ fn, p !! f = Some fn ∧ Some e2 = apply_func fn vs ∧ σ2 = σ1 ∧ efs = nil.
+  Lemma call_head_step_inv p f vs σ1 e2 σ2 :
+    head_step p (of_class Λ (ExprCall f vs)) σ1 e2 σ2 →
+    ∃ fn, p !! f = Some fn ∧ Some e2 = apply_func fn vs ∧ σ2 = σ1.
   Proof. eapply call_head_step. Qed.
   Lemma call_head_step_intro p f vs fn σ1 er :
     p !! f = Some fn →
     Some er = apply_func fn vs →
-    head_step p (of_call Λ f vs) σ1 er σ1 [].
+    head_step p (of_call Λ f vs) σ1 er σ1.
   Proof. intros ? ?. eapply call_head_step; eexists; eauto. Qed.
 
   Definition head_reducible_no_threads (p : prog Λ) (e : expr Λ) (σ : state Λ) :=
-    ∃ e' σ', head_step p e σ e' σ' [].
+    ∃ e' σ', head_step p e σ e' σ'.
   Definition head_reducible (p : prog Λ) (e : expr Λ) (σ : state Λ) :=
-    ∃ e' σ' efs, head_step p e σ e' σ' efs.
+    ∃ e' σ', head_step p e σ e' σ'.
   Definition head_irreducible (p : prog Λ) (e : expr Λ) (σ : state Λ) :=
-    ∀ e' σ' efs, ¬head_step p e σ e' σ' efs.
+    ∀ e' σ', ¬head_step p e σ e' σ'.
   Definition head_stuck (p : prog Λ) (e : expr Λ) (σ : state Λ) :=
     to_val e = None ∧ head_irreducible p e σ.
 
@@ -242,30 +234,28 @@ Section mlanguage.
   Definition sub_redexes_are_values (e : expr Λ) :=
     ∀ K e', e = fill K e' → to_val e' = None → K = empty_ectx.
 
-  Inductive prim_step (p : prog Λ) : expr Λ → state Λ → expr Λ → state Λ → list (expr Λ) → Prop :=
-    Prim_step K e1 e2 σ1 σ2 e1' e2' efs:
+  Inductive prim_step (p : prog Λ) : expr Λ → state Λ → expr Λ → state Λ → Prop :=
+    Prim_step K e1 e2 σ1 σ2 e1' e2':
       e1 = fill K e1' → e2 = fill K e2' →
-      head_step p e1' σ1 e2' σ2 efs → prim_step p e1 σ1 e2 σ2 efs.
+      head_step p e1' σ1 e2' σ2 → prim_step p e1 σ1 e2 σ2.
 
-  Lemma Prim_step' p K e1 σ1 e2 σ2 efs :
-    head_step p e1 σ1 e2 σ2 efs → prim_step p (fill K e1) σ1 (fill K e2) σ2 efs.
+  Lemma Prim_step' p K e1 σ1 e2 σ2 :
+    head_step p e1 σ1 e2 σ2 → prim_step p (fill K e1) σ1 (fill K e2) σ2.
   Proof. econstructor; eauto. Qed.
 
-  Definition reducible_no_threads (p : prog Λ) (e : expr Λ) (σ : state Λ) :=
-    ∃ e' σ', prim_step p e σ e' σ' [].
   Definition reducible (p : prog Λ) (e : expr Λ) (σ : state Λ) :=
-    ∃ e' σ' efs, prim_step p e σ e' σ' efs.
+    ∃ e' σ', prim_step p e σ e' σ'.
   Definition irreducible (p : prog Λ) (e : expr Λ) (σ : state Λ) :=
-    ∀ e' σ' efs, ¬prim_step p e σ e' σ' efs.
+    ∀ e' σ', ¬prim_step p e σ e' σ'.
   Definition stuck (p : prog Λ) (e : expr Λ) (σ : state Λ) :=
     to_val e = None ∧ irreducible p e σ.
   Definition not_stuck (p : prog Λ) (e : expr Λ) (σ : state Λ) :=
     is_Some (to_val e) ∨ reducible p e σ.
 
   (** * Some lemmas about this language *)
-  Lemma prim_step_inv p e1 e2 σ1 σ2 efs:
-    prim_step p e1 σ1 e2 σ2 efs →
-    ∃ K e1' e2', e1 = fill K e1' ∧ e2 = fill K e2' ∧ head_step p e1' σ1 e2' σ2 efs.
+  Lemma prim_step_inv p e1 e2 σ1 σ2:
+    prim_step p e1 σ1 e2 σ2 →
+    ∃ K e1' e2', e1 = fill K e1' ∧ e2 = fill K e2' ∧ head_step p e1' σ1 e2' σ2.
   Proof. inversion 1; subst; do 3 eexists; eauto. Qed.
   Lemma to_of_val v : to_val (of_val Λ v) = Some v.
   Proof. rewrite /to_val /of_val to_of_class //. Qed.
@@ -276,7 +266,7 @@ Section mlanguage.
   Qed.
   Lemma of_to_val_flip v e : of_val Λ v = e → to_val e = Some v.
   Proof. intros <-. by rewrite to_of_val. Qed.
-  Lemma val_head_stuck p e σ e' σ' efs: head_step p e σ e' σ' efs → to_val e = None.
+  Lemma val_head_stuck p e σ e' σ': head_step p e σ e' σ' → to_val e = None.
   Proof.
     destruct (to_val e) as [v|] eqn:Hval; last done.
     rewrite -(of_to_val e v) //. intros []%val_head_step.
@@ -288,7 +278,7 @@ Section mlanguage.
     - subst K. move: Hval. rewrite fill_empty. done.
     - done.
   Qed.
-  Lemma val_stuck p e σ e' σ' efs: prim_step p e σ e' σ' efs → to_val e = None.
+  Lemma val_stuck p e σ e' σ': prim_step p e σ e' σ' → to_val e = None.
   Proof.
     intros (?&?&? & -> & -> & ?%val_head_stuck)%prim_step_inv.
     apply eq_None_not_Some. by intros ?%fill_val%eq_None_not_Some.
@@ -307,9 +297,9 @@ Section mlanguage.
   Lemma not_reducible p e σ : ¬reducible p e σ ↔ irreducible p e σ.
   Proof. unfold reducible, irreducible. naive_solver. Qed.
   Lemma reducible_not_val p e σ : reducible p e σ → to_val e = None.
-  Proof. intros (?&?&?&?); eauto using val_stuck. Qed.
+  Proof. intros (?&?&?); eauto using val_stuck. Qed.
   Lemma val_irreducible p e σ : is_Some (to_val e) → irreducible p e σ.
-  Proof. intros [??] ?? ??%val_stuck. by destruct (to_val e). Qed.
+  Proof. intros [??] ? ??%val_stuck. by destruct (to_val e). Qed.
   Global Instance of_val_inj : Inj (=) (=) (@of_val _ _ Λ).
   Proof. by intros v v' Hv; apply (inj Some); rewrite -!to_of_val Hv. Qed.
   Lemma not_not_stuck p e σ : ¬not_stuck p e σ ↔ stuck p e σ.
@@ -335,36 +325,34 @@ Section mlanguage.
     head_reducible p e' σ →
     K = comp_ectx K' empty_ectx ∧ e = e'.
   Proof.
-    intros Heq (e2 & σ2 & efs & Hred) (e2' & σ2' & efs' & Hred').
+    intros Heq (e2 & σ2 & Hred) (e2' & σ2' & Hred').
     edestruct (step_by_val p K' K e' e) as [K'' HK];
       [by eauto using val_head_stuck..|].
     subst K. move: Heq. rewrite -fill_comp. intros <-%(inj (fill _)).
-    destruct (head_ctx_step_val _ _ _ _ _ _ _ Hred') as [HK''|[]%not_eq_None_Some].
+    destruct (head_ctx_step_val _ _ _ _ _ _ Hred') as [HK''|[]%not_eq_None_Some].
     - subst K''. rewrite fill_empty. done.
     - by eapply val_head_stuck.
   Qed.
 
-  Lemma head_prim_step p e1 σ1 e2 σ2 efs :
-    head_step p e1 σ1 e2 σ2 efs → prim_step p e1 σ1 e2 σ2 efs.
+  Lemma head_prim_step p e1 σ1 e2 σ2 :
+    head_step p e1 σ1 e2 σ2 → prim_step p e1 σ1 e2 σ2.
   Proof. apply Prim_step with empty_ectx; by rewrite ?fill_empty. Qed.
 
-  Lemma head_step_not_stuck p e σ e' σ' efs:
-    head_step p e σ e' σ' efs → not_stuck p e σ.
+  Lemma head_step_not_stuck p e σ e' σ':
+    head_step p e σ e' σ' → not_stuck p e σ.
   Proof. rewrite /not_stuck /reducible /=. eauto 10 using head_prim_step. Qed.
 
-  Lemma fill_prim_step p K e1 σ1 e2 σ2 efs :
-    prim_step p e1 σ1 e2 σ2 efs → prim_step p (fill K e1) σ1 (fill K e2) σ2 efs.
+  Lemma fill_prim_step p K e1 σ1 e2 σ2 :
+    prim_step p e1 σ1 e2 σ2 → prim_step p (fill K e1) σ1 (fill K e2) σ2.
   Proof.
     intros (K' & e1' & e2' & -> & -> & ?) % prim_step_inv.
     rewrite !fill_comp. by econstructor.
   Qed.
   Lemma fill_reducible p K e σ : reducible p e σ → reducible p (fill K e) σ.
   Proof.
-    intros (e'&σ'&efs&?). exists (fill K e'), σ', efs. by apply fill_prim_step.
+    intros (e'&σ'&?). exists (fill K e'), σ'. by apply fill_prim_step.
   Qed.
   Lemma head_prim_reducible p e σ : head_reducible p e σ → reducible p e σ.
-  Proof. intros (e'&σ'&efs&?). eexists e', σ', efs. by apply head_prim_step. Qed.
-  Lemma head_prim_reducible_no_threads p e σ : head_reducible_no_threads p e σ → reducible_no_threads p e σ.
   Proof. intros (e'&σ'&?). eexists e', σ'. by apply head_prim_step. Qed.
   Lemma head_prim_fill_reducible p e K σ :
     head_reducible p e σ → reducible p (fill K e) σ.
@@ -374,16 +362,16 @@ Section mlanguage.
     rewrite -not_reducible -not_head_reducible. eauto using head_prim_reducible.
   Qed.
 
-  Lemma prim_head_step p e σ e' σ' efs:
-    prim_step p e σ e' σ' efs → sub_redexes_are_values e → head_step p e σ e' σ' efs.
+  Lemma prim_head_step p e σ e' σ':
+    prim_step p e σ e' σ' → sub_redexes_are_values e → head_step p e σ e' σ'.
   Proof.
-    intros Hprim ?. destruct (prim_step_inv _ _ _ _ _ _ Hprim) as (K & e1' & e2' & -> & -> & Hstep).
+    intros Hprim ?. destruct (prim_step_inv _ _ _ _ _ Hprim) as (K & e1' & e2' & -> & -> & Hstep).
     assert (K = empty_ectx) as -> by eauto 10 using val_head_stuck.
     rewrite !fill_empty /head_reducible; eauto.
   Qed.
   Lemma prim_head_reducible p e σ :
     reducible p e σ → sub_redexes_are_values e → head_reducible p e σ.
-  Proof. intros (e'&σ'&efs&Hprim) ?. do 3 eexists; by eapply prim_head_step. Qed.
+  Proof. intros (e'&σ'&Hprim) ?. do 2 eexists; by eapply prim_head_step. Qed.
   Lemma prim_head_irreducible p e σ :
     head_irreducible p e σ → sub_redexes_are_values e → irreducible p e σ.
   Proof.
@@ -396,12 +384,12 @@ Section mlanguage.
     intros [] ?. split; first done. by apply prim_head_irreducible.
   Qed.
 
-  Lemma head_reducible_prim_step_ctx p K e1 σ1 e2 σ2 efs :
+  Lemma head_reducible_prim_step_ctx p K e1 σ1 e2 σ2 :
     head_reducible p e1 σ1 →
-    prim_step p (fill K e1) σ1 e2 σ2 efs →
-    ∃ e2', e2 = fill K e2' ∧ head_step p e1 σ1 e2' σ2 efs.
+    prim_step p (fill K e1) σ1 e2 σ2 →
+    ∃ e2', e2 = fill K e2' ∧ head_step p e1 σ1 e2' σ2.
   Proof.
-    intros (e2''&σ2''&efs'&HhstepK) (K' & e1' & e2' & HKe1 & -> & Hstep) % prim_step_inv.
+    intros (e2''&σ2''&HhstepK) (K' & e1' & e2' & HKe1 & -> & Hstep) % prim_step_inv.
     edestruct (step_by_val p K) as [K'' ?];
       eauto using val_head_stuck; simplify_eq/=.
     rewrite -fill_comp in HKe1; simplify_eq.
@@ -411,10 +399,10 @@ Section mlanguage.
     - apply val_head_stuck in Hstep; simplify_eq.
   Qed.
 
-  Lemma head_reducible_prim_step p e1 σ1 e2 σ2 efs :
+  Lemma head_reducible_prim_step p e1 σ1 e2 σ2 :
     head_reducible p e1 σ1 →
-    prim_step p e1 σ1 e2 σ2 efs →
-    head_step p e1 σ1 e2 σ2 efs.
+    prim_step p e1 σ1 e2 σ2 →
+    head_step p e1 σ1 e2 σ2.
   Proof.
     intros.
     edestruct (head_reducible_prim_step_ctx p empty_ectx) as (?&?&?);
@@ -426,8 +414,8 @@ Section mlanguage.
   Proof.
     intros Hstuck; split.
     + apply fill_not_val, Hstuck.
-    + intros e'' σ'' efs (K_redex &e1 &e2 &Heq &-> &Hhead)%prim_step_inv.
-      edestruct (step_by_val P K K_redex _ _ _ _ _ _ Heq ltac:(apply Hstuck) Hhead) as (K'' & ->).
+    + intros e'' σ'' (K_redex &e1 &e2 &Heq &-> &Hhead)%prim_step_inv.
+      edestruct (step_by_val P K K_redex _ _ _ _ _ Heq ltac:(apply Hstuck) Hhead) as (K'' & ->).
       rewrite -fill_comp in Heq. apply fill_inj in Heq as ->.
       eapply (proj2 Hstuck). econstructor; eauto.
   Qed.
@@ -436,17 +424,17 @@ Section mlanguage.
   Proof.
     intros [Hval | Hred].
     - left. by eapply fill_val.
-    - destruct Hred as (e' & σ' & efs & (K_redex &e1 &e2 &Heq &-> &Hhead)%prim_step_inv).
+    - destruct Hred as (e' & σ' & (K_redex &e1 &e2 &Heq &-> &Hhead)%prim_step_inv).
       destruct (decide (to_val e = None)) as [Hnval | Hval]; first last.
       { left. destruct (to_val e) as [v | ]; by eauto. }
-      edestruct (step_by_val P K K_redex _ _ _ _ _ _ Heq Hnval Hhead) as (K'' & ->).
+      edestruct (step_by_val P K K_redex _ _ _ _ _ Heq Hnval Hhead) as (K'' & ->).
       rewrite -fill_comp in Heq. apply fill_inj in Heq as ->.
-      right. eexists _, _, _. econstructor; eauto.
+      right. eexists _, _. econstructor; eauto.
   Qed.
 
-  Lemma prim_step_call_inv p K f vs e' σ σ' efs :
-    prim_step p (fill K (of_call Λ f vs)) σ e' σ' efs →
-    ∃ er fn, Some er = apply_func fn vs ∧ p !! f = Some fn ∧ e' = fill K er ∧ σ' = σ ∧ efs = [].
+  Lemma prim_step_call_inv p K f vs e' σ σ' :
+    prim_step p (fill K (of_call Λ f vs)) σ e' σ' →
+    ∃ er fn, Some er = apply_func fn vs ∧ p !! f = Some fn ∧ e' = fill K er ∧ σ' = σ.
   Proof.
     intros (K' & e1 & e2 & Hctx & -> & Hstep)%prim_step_inv.
     eapply step_by_val in Hstep as H'; eauto; last apply to_val_of_call.
@@ -455,13 +443,13 @@ Section mlanguage.
     destruct (fill_class K'' e1) as [->|Hval].
     - apply is_call_is_class. erewrite of_to_call_flip; eauto.
     - rewrite fill_empty in Hctx. subst e1. exists e2.
-      apply call_head_step_inv in Hstep as (fn & ? & -> & -> & ->).
+      apply call_head_step_inv in Hstep as (fn & ? & -> & ->).
       exists fn. rewrite -fill_comp fill_empty. naive_solver.
     - unfold is_Some in Hval. erewrite val_head_stuck in Hval; naive_solver.
   Qed.
 
-  Lemma val_prim_step p v σ e' σ' efs :
-   ¬ prim_step p (of_val Λ v) σ e' σ' efs.
+  Lemma val_prim_step p v σ e' σ':
+   ¬ prim_step p (of_val Λ v) σ e' σ'.
   Proof.
     intros (K & e1' & e2' & Heq & -> & Hstep') % prim_step_inv.
     edestruct (fill_val K e1') as (v1''& ?).
@@ -470,10 +458,10 @@ Section mlanguage.
     erewrite <-(of_to_val e1') in Hstep'; eauto.
   Qed.
 
-  Lemma fill_reducible_prim_step p e e' σ σ' K efs :
-    reducible p e σ → prim_step p (fill K e) σ e' σ' efs → ∃ e'', e' = fill K e'' ∧ prim_step p e σ e'' σ' efs.
+  Lemma fill_reducible_prim_step p e e' σ σ' K :
+    reducible p e σ → prim_step p (fill K e) σ e' σ' → ∃ e'', e' = fill K e'' ∧ prim_step p e σ e'' σ'.
   Proof.
-    intros (e1 & σ1 & efs' & (K'' & e1'' & e2'' & ->  & -> & Hhead) % prim_step_inv) Hprim.
+    intros (e1 & σ1 & (K'' & e1'' & e2'' & ->  & -> & Hhead) % prim_step_inv) Hprim.
     rewrite fill_comp in Hprim.
     eapply head_reducible_prim_step_ctx in Hprim as (e1' & -> & Hhead'); last by rewrite /head_reducible; eauto.
     eexists. rewrite -fill_comp; by eauto using Prim_step'.
@@ -481,32 +469,18 @@ Section mlanguage.
 
   Lemma reducible_fill p e σ K : reducible p e σ → reducible p (fill K e) σ.
   Proof.
-  intros (e' & σ' & efs & Hs).
-  inversion Hs; subst.
-  eexists (fill (comp_ectx K K0) e2'), σ', efs. econstructor. 1: rewrite fill_comp; reflexivity. 1: reflexivity. apply H1.
-  Qed.
-
-  Lemma reducible_no_threads_fill p e σ K : reducible_no_threads p e σ → reducible_no_threads p (fill K e) σ.
-  Proof.
   intros (e' & σ' & Hs).
   inversion Hs; subst.
   eexists (fill (comp_ectx K K0) e2'), σ'. econstructor. 1: rewrite fill_comp; reflexivity. 1: reflexivity. apply H1.
   Qed.
 
-
-  Lemma reducible_no_threads_reducible p e σ K : reducible_no_threads p e σ → reducible p e σ.
-  Proof.
-  intros (e' & σ' & Hs).
-  now exists e', σ', [].
-  Qed.
-
-  Lemma fill_step_inv K p e1' σ1 e2 σ2 efs :
-    to_val e1' = None → prim_step p (fill K e1') σ1 e2 σ2 efs →
-    ∃ e2', e2 = fill K e2' ∧ prim_step p e1' σ1 e2' σ2 efs.
+  Lemma fill_step_inv K p e1' σ1 e2 σ2 :
+    to_val e1' = None → prim_step p (fill K e1') σ1 e2 σ2 →
+    ∃ e2', e2 = fill K e2' ∧ prim_step p e1' σ1 e2' σ2.
   Proof.
     intros H1 H2.
     inversion H2; subst.
-    destruct (step_by_val _ _ _ _ _ _ _ _ _ H H1 H3) as (K'' & ->).
+    destruct (step_by_val _ _ _ _ _ _ _ _ H H1 H3) as (K'' & ->).
     rewrite <- fill_comp in *.
     apply fill_inj in H. subst. eexists; split; first done.
     by econstructor.
@@ -514,657 +488,19 @@ Section mlanguage.
 
   Lemma fill_inv p K e σ : to_val e = None -> reducible p (fill K e) σ -> reducible p e σ.
   Proof.
-    intros H1 (e'&σ'&efs&(e2'&->&H2)%fill_step_inv). 2:easy.
-    exists e2',σ',efs. easy.
+    intros H1 (e'&σ'&(e2'&->&H2)%fill_step_inv). 2:easy.
+    exists e2',σ'. easy.
   Qed.
 
-  Lemma head_call_pure p f vs σ e2 σ' σ2 efs : 
-    head_step p (of_class Λ (ExprCall f vs)) σ e2 σ' efs -> head_step p (of_class Λ (ExprCall f vs)) σ2 e2 σ2 [].
+  Lemma head_call_pure p f vs σ e2 σ' σ2 :
+    head_step p (of_class Λ (ExprCall f vs)) σ e2 σ' -> head_step p (of_class Λ (ExprCall f vs)) σ2 e2 σ2.
   Proof.
     intros (fn & H1 & H2 & H3)%call_head_step. apply call_head_step.
     exists fn. repeat split; easy.
   Qed.
 
-  (** Lifting of steps to thread pools *)
-  Definition tpool {val public_state} (Λ : mlanguage val public_state) := list (expr Λ).
-  Implicit Types (T: tpool Λ).  (* thread pools *)
-  Implicit Types (I J: list nat).       (* traces *)
-  Implicit Types (O: gset nat).       (* trace sets *)
-
-  Inductive pool_step (p: prog Λ): tpool Λ → state Λ → nat → tpool Λ → state Λ → Prop :=
-    | Pool_step i T_l e e' T_r efs σ σ':
-        prim_step p e σ e' σ' efs →
-        i = length T_l →
-        pool_step p (T_l ++ e :: T_r) σ i (T_l ++ e' :: T_r ++ efs) σ'.
-
-  Inductive pool_steps (p: prog Λ): tpool Λ → state Λ → list nat → tpool Λ → state Λ → Prop :=
-    | Pool_steps_refl T σ: pool_steps p T σ [] T σ
-    | Pool_steps_step T T' T'' σ σ' σ'' i I:
-      pool_step p T σ i T' σ' →
-      pool_steps p T' σ' I T'' σ'' →
-      pool_steps p T σ (i:: I) T'' σ''.
-
-
-  Lemma pool_step_iff p T σ i T' σ':
-    pool_step p T σ i T' σ' ↔
-    (∃ e e' efs, prim_step p e σ e' σ' efs ∧ T !! i = Some e ∧ T' = <[i := e']> T ++ efs).
-  Proof.
-    split.
-    - destruct 1 as [i T_l e e' T_r efs σ σ' Hstep Hlen]; subst.
-      exists e, e', efs. split; first done.
-      rewrite list_lookup_middle; last done.
-      split; first done.
-      replace (length T_l) with (length T_l + 0) by lia.
-      rewrite insert_app_r; simpl.
-      by rewrite -app_assoc.
-    - intros (e & e' & efs & Hstep & Hlook & ->).
-      replace T with (take i T ++ e :: drop (S i) T); last by eapply take_drop_middle.
-      assert (i = length (take i T)).
-      { rewrite take_length_le; first lia. eapply lookup_lt_Some in Hlook. lia. }
-      replace i with (length (take i T) + 0) at 4 by lia.
-      rewrite insert_app_r. simpl.
-      rewrite -app_assoc; simpl.
-      econstructor; auto.
-  Qed.
-
-  Lemma pool_step_value_preservation p v T σ i j T' σ':
-    pool_step p T σ j T' σ' →
-    T !! i = Some (of_val Λ v) →
-    T' !! i = Some (of_val Λ v).
-  Proof.
-    rewrite pool_step_iff.
-    destruct 1 as (e1 & e2 & efs & Hstep & Hpre & Hpost).
-    intros Hlook. destruct (decide (i = j)); subst.
-    - pose proof val_prim_step. by naive_solver.
-    - eapply lookup_app_l_Some.
-      rewrite list_lookup_insert_ne; done.
-  Qed.
-
-  Lemma pool_steps_value_preservation p v T σ i J T' σ':
-    pool_steps p T σ J T' σ' →
-    T !! i = Some (of_val Λ v) →
-    T' !! i = Some (of_val Λ v).
-  Proof.
-    induction 1; eauto using pool_step_value_preservation.
-  Qed.
-
-  Lemma pool_steps_single p T σ i T' σ':
-    pool_step p T σ i T' σ' ↔
-    pool_steps p T σ [i] T' σ'.
-  Proof.
-    split.
-    - intros Hstep; eauto using pool_steps.
-    - inversion 1 as [|????????? Hsteps]. subst; inversion Hsteps; by subst.
-  Qed.
-
-  Lemma pool_steps_trans p T T' T'' σ σ' σ'' I J:
-    pool_steps p T σ I T' σ' →
-    pool_steps p T' σ' J T'' σ'' →
-    pool_steps p T σ (I ++ J) T'' σ''.
-  Proof.
-    induction 1; simpl; eauto using pool_steps.
-  Qed.
-
-
-  (** Threads in a thread pool *)
-  Definition threads T :=
-    list_to_set (C := gset nat) (seq 0 (length T)).
-
-  Lemma threads_spec T i:
-    i ∈ threads T ↔ ∃ e, T !! i = Some e.
-  Proof.
-    rewrite elem_of_list_to_set elem_of_seq.
-    split.
-    - intros [_ Hlt]. eapply lookup_lt_is_Some_2. lia.
-    - intros ? % lookup_lt_is_Some_1. lia.
-  Qed.
-
-  Lemma threads_insert T i e:
-    threads T ⊆ threads (<[i:=e]> T).
-  Proof.
-    intros j [e' Hlook]%threads_spec.
-    eapply threads_spec.
-    destruct (decide (i = j)).
-    - subst; exists e.
-      eapply list_lookup_insert, lookup_lt_Some, Hlook.
-    - rewrite list_lookup_insert_ne; last done. by exists e'.
-  Qed.
-
-  Lemma threads_app T T':
-    threads T ⊆ threads (T ++ T').
-  Proof.
-    intros j (e & Hlook)%threads_spec.
-    eapply threads_spec. exists e.
-    eapply lookup_app_l_Some, Hlook.
-  Qed.
-
-  (* a prim_step does the following mutation to the thread pool *)
-  Lemma threads_prim_step e' T' i T :
-    threads T ⊆ threads (<[i := e']> T ++ T').
-  Proof.
-    etrans; last eapply threads_app.
-    eapply threads_insert.
-  Qed.
-
-  Lemma threads_pool_step p T σ i T' σ' :
-    pool_step p T σ i T' σ' →
-    threads T ⊆ threads T'.
-  Proof.
-    rewrite pool_step_iff; intros (e & e' & efs & Hstep & Hlook & ->).
-    eapply threads_prim_step.
-  Qed.
-
-  Lemma threads_pool_steps p T σ I T' σ' :
-    pool_steps p T σ I T' σ' →
-    threads T ⊆ threads T'.
-  Proof.
-    induction 1; first done.
-    etrans; first eapply threads_pool_step; eauto.
-  Qed.
-
-  (** Reaching Stuck State Λs/Safety *)
-  (* a thread pool has undefined behavior, if one of its threads has undefined behavior. *)
-  Definition not_stuck_pool p T σ := ∀ e i, T !! i = Some e → not_stuck p e σ.
-  Definition pool_safe p T σ := ∀ T' σ' I, pool_steps p T σ I T' σ' → not_stuck_pool p T' σ'.
-  Definition stuck_pool p T σ := (∃ e i, T !! i = Some e ∧ stuck p e σ).
-  Definition pool_reach_stuck p T σ :=
-    ∃ T' σ' I, pool_steps p T σ I T' σ' ∧ stuck_pool p T' σ'.
-
-  Lemma stuck_pool_not_not_stuck_pool p T σ :
-    stuck_pool p T σ → ¬ not_stuck_pool p T σ.
-  Proof.
-    intros (e & i & Hlookup & [Hnval Hirred]) Hnot.
-    apply Hnot in Hlookup as [Hval | Hred].
-    - rewrite Hnval in Hval. destruct Hval as [? [=]].
-    - apply not_reducible in Hirred. done.
-  Qed.
-
-  Lemma pool_reach_stuck_not_safe p T σ :
-    pool_reach_stuck p T σ → ¬ pool_safe p T σ.
-  Proof.
-    intros (T' & σ' & I & Hsteps & Hstuck) Hsafe.
-    apply Hsafe in Hsteps. eapply stuck_pool_not_not_stuck_pool; done.
-  Qed.
-
-  Lemma pool_step_singleton p e σ i σ' T:
-    pool_step p [e] σ i T σ' ↔
-    (∃ e' efs, prim_step p e σ e' σ' efs ∧ T = e' :: efs ∧ i = 0).
-  Proof.
-    rewrite pool_step_iff. destruct i; simpl; naive_solver.
-  Qed.
-
-  Lemma pool_steps_values p T σ I T' σ' :
-    pool_steps p T σ I T' σ' →
-    (∀ e, e ∈ T → is_Some (to_val e)) →
-    T' = T ∧ σ = σ' ∧ I = [].
-  Proof.
-    destruct 1 as [|T T' T'' σ σ' σ'' i I Hstep Hsteps]; eauto.
-    intros Hvals.
-    eapply pool_step_iff in Hstep as (e & e' & efs & Hstep & Hlook & Hupd).
-    feed pose proof (Hvals e) as Irr; first by eapply elem_of_list_lookup_2.
-    exfalso; eapply val_irreducible; eauto.
-  Qed.
-
-  Lemma pool_step_fill_context p e K i j σ σ' T T':
-    pool_step p T σ j T' σ' →
-    T !! i = Some e →
-    ∃ e', T' !! i = Some e' ∧
-    pool_step p (<[i := fill K e]> T) σ j (<[i := fill K e']> T') σ'.
-  Proof.
-    rewrite pool_step_iff; intros (e1 & e2 & efs & Hprim & Hlook & Hupd) Hlook1.
-    destruct (decide (i = j)).
-    - subst. assert (<[j:=e2]> T !! j = Some e2) as Hlook2.
-      { eapply list_lookup_insert, lookup_lt_Some, Hlook. }
-      exists e2; split; first eapply lookup_app_l_Some, Hlook2.
-      rewrite insert_app_l; last by eapply lookup_lt_Some, Hlook2.
-      rewrite list_insert_insert. assert (e1 = e) as -> by naive_solver.
-      eapply pool_step_iff; exists (fill K e), (fill K e2), efs.
-      split; first by eapply fill_prim_step.
-      split; first eapply list_lookup_insert, lookup_lt_Some, Hlook.
-      by rewrite list_insert_insert.
-    - exists e. rewrite Hupd.
-      rewrite (lookup_app_l_Some _ _ _ e);
-        last by rewrite list_lookup_insert_ne //.
-      rewrite insert_app_l;
-        last (eapply lookup_lt_Some; rewrite list_lookup_insert_ne //).
-      split; first done.
-      rewrite list_insert_commute //.
-      eapply pool_step_iff; exists e1, e2, efs.
-      split; first done.
-      split; first rewrite list_lookup_insert_ne //.
-      done.
-  Qed.
-
-  Lemma pool_steps_fill_context p e K i I σ σ' T T':
-    pool_steps p T σ I T' σ' →
-    T !! i = Some e →
-    ∃ e', T' !! i = Some e' ∧
-    pool_steps p (<[i := fill K e]> T) σ I (<[i := fill K e']> T') σ'.
-  Proof.
-    induction 1 as [T σ|T T' T'' σ σ' σ'' j I Hstep Hsteps IH] in e.
-    - eauto 10 using pool_steps.
-    - intros Hlook.
-      eapply pool_step_fill_context in Hlook as (e' & Hlook' & Hstep'); last done.
-      eapply IH in Hlook' as (e'' & Hlook'' & Hstep'').
-      eauto 10 using pool_steps.
-  Qed.
-
-  Lemma pool_steps_safe p T I T' σ σ':
-    pool_steps p T σ I T' σ' → pool_safe p T σ → pool_safe p T' σ'.
-  Proof.
-    intros Hs1 Hsafe T'' σ'' I' Hsteps. eapply Hsafe. eapply pool_steps_trans; done.
-  Qed.
-
-  Lemma pool_safe_insert_fill p T i e σ K :
-    T !! i = Some e →
-    pool_safe p (<[i := fill K e]> T) σ →
-    pool_safe p T σ.
-  Proof.
-    intros Hlook Hsafe T' σ' I Hsteps.
-    eapply (pool_steps_fill_context _ _ K) in Hsteps as (e' & Hlook' & Hsteps); last done.
-    intros e'' j He''.
-    destruct (decide (i = j)) as [-> | Hneq].
-    - assert (e'' = e') as -> by naive_solver.
-      eapply fill_not_stuck. eapply Hsafe; first done.
-      eapply list_lookup_insert, lookup_lt_Some, Hlook'.
-    - eapply Hsafe; first done. rewrite list_lookup_insert_ne //.
-  Qed.
-
-  Lemma fill_reach_stuck_pool p T i e σ K :
-    T !! i = Some e →
-    pool_reach_stuck p T σ →
-    pool_reach_stuck p (<[i := fill K e]> T) σ.
-  Proof.
-    intros Hlook (T' & σ' & I & Hsteps & Hstuck).
-    eapply (pool_steps_fill_context _ _ K) in Hsteps as (e' & Hlook' & Hsteps); last done.
-    exists (<[i:=fill K e']> T'), σ', I; split; first done.
-    destruct Hstuck as (e'' & j & Hlook'' & Hstuck).
-    destruct (decide (i = j)).
-    - subst. exists (fill K e'), j. assert (e'' = e') as -> by naive_solver.
-      split; first eapply list_lookup_insert, lookup_lt_Some, Hlook'.
-      eapply fill_stuck, Hstuck.
-    - exists e'', j. rewrite list_lookup_insert_ne //.
-  Qed.
-
-  Lemma pool_steps_reach_stuck p T I T' σ σ':
-    pool_steps p T σ I T' σ' → pool_reach_stuck p T' σ' → pool_reach_stuck p T σ.
-  Proof.
-    intros H (e'' & σ'' & J & Hstep & Hstuck).
-    exists e'', σ'', (I ++ J). split; last assumption.
-    by eapply pool_steps_trans.
-  Qed.
-
-  Lemma pool_safe_call_in_prg p K T T' i I σ σ' f vs:
-    pool_safe p T σ →
-    pool_steps p T σ I T' σ' →
-    T' !! i = Some (fill K (of_call Λ f vs)) →
-    ∃ fn', p !! f = Some fn'.
-  Proof.
-    destruct (p !! f) as [fn'|] eqn: Hloook; first by eauto.
-    intros Hsafe Hsteps Hlook. exfalso.
-    apply Hsafe in Hsteps. apply Hsteps in Hlook.
-    apply fill_not_stuck in Hlook as [Hval | Hred].
-    - rewrite to_val_of_call in Hval. destruct Hval as [? [=]].
-    - destruct Hred as (e'' & σ'' & efs & Hstep).
-      pose proof (prim_step_call_inv p empty_ectx f vs e'' σ' σ'' efs) as Hinv.
-      rewrite fill_empty in Hinv.
-      eapply Hinv in Hstep as (x_f & e_f & _ & Hprg & _). naive_solver.
-  Qed.
-
-  (** Some theory for sub-pools
-      (needed for the single-thread "reach stuck" further down) *)
-  Lemma pool_step_sub_pool p T1 T1' σ i T2 σ' :
-    pool_step p T1 σ i T1' σ' →
-    T1 ⊆+ T2 →
-    ∃ T2' j, T1' ⊆+ T2' ∧ pool_step p T2 σ j T2' σ'.
-  Proof.
-    intros (e & e' & efs & Hstep & Hlook & ->)%pool_step_iff Hsub.
-    eapply lookup_submseteq in Hsub as Hidx; last done.
-    destruct Hidx as (j & Hlook').
-    exists (<[j := e']> T2 ++ efs), j.
-    split; last (apply pool_step_iff; eauto 10).
-    eapply submseteq_app; last done.
-    eapply submseteq_insert; eauto.
-  Qed.
-
-  Lemma pool_steps_sub_pool p T1 T1' σ I T2 σ' :
-    pool_steps p T1 σ I T1' σ' →
-    T1 ⊆+ T2 →
-    ∃ T2' J, T1' ⊆+ T2' ∧ pool_steps p T2 σ J T2' σ'.
-  Proof.
-    induction 1 as [|T1 T1' T1'' σ σ' σ'' i I Hstep Hsteps IH] in T2; first by eauto using pool_steps.
-    intros Hsub; eapply pool_step_sub_pool in Hstep as (T2' & j & Hpool & Hstep); last done.
-    edestruct IH as (? & ? & ? & ?); eauto 10 using pool_steps.
-  Qed.
-
-  Lemma pool_safe_sub_pool p T1 T2 σ :
-    pool_safe p T2 σ →
-    T1 ⊆+ T2 →
-    pool_safe p T1 σ.
-  Proof.
-    intros Hsafe Hsub T' σ' I Hsteps e i He.
-    eapply pool_steps_sub_pool in Hsteps as (T2' & J & Hsub' & Hsteps'); last done.
-    eapply lookup_submseteq in Hsub' as (j & Hlook'); last done.
-    eapply Hsafe; done.
-  Qed.
-
-  Lemma pool_reach_stuck_sub_pool p T1 T2 σ:
-    pool_reach_stuck p T1 σ →
-    T1 ⊆+ T2 →
-    pool_reach_stuck p T2 σ.
-  Proof.
-    intros (T1' & σ' & I & Hsteps & Hstuck) Hsub.
-    eapply pool_steps_sub_pool in Hsteps as (T2' & J & Hsub' & Hsteps'); last done.
-    exists T2', σ', J; split; first done.
-    destruct Hstuck as (e & i & Hlook & Hstuck).
-    eapply lookup_submseteq in Hsub' as (j & Hlook'); last done.
-    exists e, j; split; eauto.
-  Qed.
-
-  (** we define the one-thread versions of the above pool notions and lemmas *)
-  Definition reach_stuck p e σ := pool_reach_stuck p [e] σ.
-  Definition safe p e σ := pool_safe p [e] σ.
-  Definition step_no_fork p e σ e' σ' := prim_step p e σ e' σ' [].
-  Inductive steps_no_fork (p: prog Λ): expr Λ → state Λ → expr Λ → state Λ → Prop :=
-    | no_forks_refl e σ: steps_no_fork p e σ e σ
-    | no_forks_step e e' e'' σ σ' σ'':
-      step_no_fork p e σ e' σ' →
-      steps_no_fork p e' σ' e'' σ'' →
-      steps_no_fork p e σ e'' σ''.
-
-  Lemma pool_safe_threads_safe p T σ i e:
-    pool_safe p T σ →
-    T !! i = Some e →
-    safe p e σ.
-  Proof.
-    intros Hsafe Hlook. eapply pool_safe_sub_pool; first done.
-    eapply singleton_submseteq_l.
-    apply elem_of_list_lookup. eauto.
-  Qed.
-
-  Lemma pool_reach_stuck_reach_stuck p e σ i T:
-    reach_stuck p e σ →
-    T !! i = Some e →
-    pool_reach_stuck p T σ.
-  Proof.
-    intros Hstuck Hlook.
-    eapply pool_reach_stuck_sub_pool; first apply Hstuck.
-    eapply singleton_submseteq_l.
-    apply elem_of_list_lookup. eauto.
-  Qed.
-
-  Lemma stuck_reach_stuck P e σ:
-    stuck P e σ → reach_stuck P e σ.
-  Proof. intros Hs; exists [e], σ, []. split; [constructor|]. by eexists _, 0. Qed.
-
-  Lemma fill_no_fork p e e' σ σ' K :
-    step_no_fork p e σ e' σ' → step_no_fork p (fill K e) σ (fill K e') σ'.
-  Proof.
-    intros ?; by eapply fill_prim_step.
-  Qed.
-
-  Lemma fill_no_forks p e e' σ σ' K :
-    steps_no_fork p e σ e' σ' → steps_no_fork p (fill K e) σ (fill K e') σ'.
-  Proof.
-    induction 1; eauto using steps_no_fork, fill_no_fork.
-  Qed.
-
-  Lemma fill_reach_stuck p e σ K :
-    reach_stuck p e σ → reach_stuck p (fill K e) σ.
-  Proof.
-    intros Hreach; eapply (fill_reach_stuck_pool _ [e] 0); done.
-  Qed.
-
-  Lemma fill_safe p e σ K :
-    safe p (fill K e) σ → safe p e σ.
-  Proof.
-    intros Hsafe. eapply (pool_safe_insert_fill _ [e] 0); done.
-  Qed.
-
-  Lemma no_forks_pool_steps_single_thread p e σ e' σ':
-    steps_no_fork p e σ e' σ' →
-    (∃ I, pool_steps p [e] σ I [e'] σ').
-  Proof.
-    induction 1 as [|e e' e'' σ σ' σ'' step_no_fork _ IH]; eauto using pool_steps.
-    destruct IH as (I & Hsteps). exists (0 :: I).
-    econstructor; first eapply pool_step_singleton; eauto 10.
-  Qed.
-
-  Lemma prim_step_pool_step T i p e σ e' σ' efs :
-    prim_step p e σ e' σ' efs →
-    T !! i = Some e →
-    pool_step p T σ i (<[i := e']> T ++ efs) σ'.
-  Proof.
-    intros ??. eapply pool_step_iff. eauto 10.
-  Qed.
-
-  Lemma no_fork_pool_step T i p e σ e' σ' :
-    step_no_fork p e σ e' σ' →
-    T !! i = Some e →
-    pool_step p T σ i (<[i := e']> T) σ'.
-  Proof.
-    intros Hnf Hlook. eapply prim_step_pool_step in Hnf; eauto.
-    by rewrite right_id in Hnf.
-  Qed.
-
-  Lemma no_forks_pool_steps T i p e σ e' σ':
-    steps_no_fork p e σ e' σ' →
-    T !! i = Some e →
-    ∃ I, pool_steps p T σ I (<[i := e']> T) σ' ∧ ((list_to_set I: gset nat) ⊆ {[i]}).
-  Proof.
-    induction 1 as [|e e' e'' σ σ' σ'' Hstep Hsteps IH] in T; intros Hlook.
-    - exists []. rewrite list_insert_id //. split; first constructor.
-      set_solver.
-    - eapply no_fork_pool_step in Hstep; last done.
-      destruct (IH (<[i := e']> T)) as (I & Hsteps' & Hsub').
-      { eapply list_lookup_insert, lookup_lt_Some, Hlook. }
-      exists (i :: I). split; last set_solver.
-      rewrite list_insert_insert in Hsteps'.
-      econstructor; done.
-  Qed.
-
-
-  Lemma no_forks_then_prim_step_pool_steps T i p e σ e' σ' e'' σ'' efs:
-    steps_no_fork p e σ e' σ' →
-    prim_step p e' σ' e'' σ'' efs →
-    T !! i = Some e →
-    ∃ I, pool_steps p T σ I (<[i := e'']> T ++ efs) σ'' ∧ ((list_to_set I: gset nat) = {[i]}).
-  Proof.
-    intros Hnfs Hprim Hlook. eapply no_forks_pool_steps in Hnfs as (I & Hsteps & Hsub); last done.
-    exists (I ++ [i]); split; last set_solver.
-    eapply pool_steps_trans; eauto. eapply pool_steps_single.
-    rewrite -(list_insert_insert T i e'' e').
-    eapply prim_step_pool_step; first done.
-    eapply list_lookup_insert, lookup_lt_Some, Hlook.
-  Qed.
-
-  Lemma pool_reach_stuck_no_forks π p T e e' σ σ':
-    T !! π = Some e →
-    steps_no_fork p e σ e' σ' → pool_reach_stuck p (<[π := e']>T) σ' → pool_reach_stuck p T σ.
-  Proof.
-    intros HT Hnfs Hrs.
-    pose proof no_forks_pool_steps _ _ _ _ _ _ _ Hnfs HT as [? [??]].
-    by apply: pool_steps_reach_stuck.
-  Qed.
-
-  Lemma pool_safe_no_forks p T e σ i e' σ':
-    pool_safe p T σ →
-    T !! i = Some e →
-    steps_no_fork p e σ e' σ' →
-    pool_safe p (<[i := e']>T) σ'.
-  Proof.
-    intros Hsafe HT Hnfs.
-    pose proof no_forks_pool_steps _ _ _ _ _ _ _ Hnfs HT as [? [??]].
-    by apply: pool_steps_safe.
-  Qed.
-
-  Lemma safe_call_in_prg p K e σ σ' f vs:
-    safe p e σ →
-    steps_no_fork p e σ (fill K (of_call Λ f vs)) σ' →
-    ∃ fn, p !! f = Some fn.
-  Proof.
-    intros H1 (I & Hsteps)%no_forks_pool_steps_single_thread.
-    eapply (pool_safe_call_in_prg _ _ _ _ 0) in Hsteps; eauto.
-  Qed.
-
-  Lemma no_forks_val p v σ e' σ' :
-    steps_no_fork p (of_val Λ v) σ e' σ' → e' = of_val Λ v ∧ σ' = σ.
-  Proof.
-    intros (I & Hsteps)%no_forks_pool_steps_single_thread.
-    eapply pool_steps_values in Hsteps; first naive_solver.
-    intros e Hel. assert (e = of_val Λ v) as -> by set_solver.
-    rewrite to_of_val; eauto.
-  Qed.
-
-  Lemma val_safe p v σ : safe p (of_val Λ v) σ.
-  Proof.
-    intros T' σ' I Hsteps e i Hlookup.
-    eapply pool_steps_values in Hsteps as (-> & -> & ->); last first.
-    { intros e' Hel. assert (e' = of_val Λ v) as -> by set_solver.
-      rewrite to_of_val; eauto. }
-    rewrite list_lookup_singleton in Hlookup. destruct i; last done.
-    assert (e = of_val Λ v) as -> by congruence.
-    left. rewrite to_of_val. eauto.
-  Qed.
-
-  Lemma reach_stuck_no_forks P e σ e' σ':
-    reach_stuck P e' σ' → steps_no_fork P e σ e' σ' →  reach_stuck P e σ.
-  Proof.
-    intros (T'' & σ'' & I & Hsteps & Hstuck) (J & Hnfs)%no_forks_pool_steps_single_thread.
-    exists T'', σ'', (J ++ I). split; last done.
-    by eapply pool_steps_trans.
-  Qed.
-
-  Lemma safe_no_forks P e σ e' σ':
-    safe P e σ → steps_no_fork P e σ e' σ' → safe P e' σ'.
-  Proof.
-    intros Hsafe (J & Hnfs)%no_forks_pool_steps_single_thread T'' σ'' I Hsteps e'' i Hlookup.
-    eapply Hsafe. { eapply pool_steps_trans; done. }
-    done.
-  Qed.
-
-  Lemma no_forks_trans P e σ e' σ' e'' σ'':
-    steps_no_fork P e σ e' σ' → steps_no_fork P e' σ' e'' σ'' → steps_no_fork P e σ e'' σ''.
-  Proof.
-    induction 1; eauto using steps_no_fork.
-  Qed.
-
-  Lemma no_forks_inv_r P e σ e' σ':
-    steps_no_fork P e σ e' σ' → (e' = e ∧ σ' = σ) ∨ (∃ e'' σ'', steps_no_fork P e σ e'' σ'' ∧ step_no_fork P e'' σ'' e' σ').
-  Proof.
-    induction 1 as [|e e' e'' σ σ' σ'' Hstep Hsteps IH]; first by eauto.
-    destruct IH as [(-> & ->)|(e''' & σ''' & Hnfs & Hnf)]; eauto 10 using steps_no_fork.
-  Qed.
-
 End mlanguage.
 
-
-Section safe_reach.
-  Context {val public_state} {Λ : mlanguage val public_state}.
-
-  (** [post_in_ectx] allows ignoring arbitrary evaluation contexts
-  around e and is meant as a combinator for the postcondition of
-  [safe_reach]. *)
-  Definition post_in_ectx (Φ : expr Λ → state Λ → Prop) (e : expr Λ) (σ : state Λ) : Prop :=
-    ∃ Ks e', e = fill Ks e' ∧ Φ e' σ.
-
-  Lemma post_in_ectx_intro (Φ : expr Λ → state Λ → Prop) e σ:
-    Φ e σ →
-    post_in_ectx Φ e σ.
-  Proof. eexists empty_ectx, e. rewrite fill_empty. naive_solver. Qed.
-
-  Lemma post_in_ectx_mono (Φ1 Φ2 : expr Λ → state Λ → Prop) e σ:
-    post_in_ectx Φ1 e σ →
-    (∀ e σ, Φ1 e σ → Φ2 e σ) →
-    post_in_ectx Φ2 e σ.
-  Proof. move => [?[?[??]]] ?. eexists _, _. naive_solver. Qed.
-
-  (** [safe_reach P e σ Φ] says that starting from e in state Λ σ,
-    under the assumption that this is a [safe] configuration,
-     one can reach e' in σ' such that Φ e' σ' holds. *)
-  Definition safe_reach (P : prog Λ) (e : expr Λ) (σ : state Λ) (Φ : expr Λ → state Λ → Prop) : Prop :=
-    safe P e σ → ∃ e' σ', steps_no_fork P e σ e' σ' ∧ Φ e' σ'.
-
-  Lemma safe_reach_refl p e σ (Φ : _ → _ → Prop):
-    Φ e σ → safe_reach p e σ Φ.
-  Proof. move => ? ?. eexists _, _ => /=. split; [|done]. by apply: no_forks_refl. Qed.
-
-  Lemma safe_reach_mono p e σ (Φ1 Φ2 : _ → _ → Prop):
-    safe_reach p e σ Φ1 → (∀ e σ, Φ1 e σ → Φ2 e σ) → safe_reach p e σ Φ2.
-  Proof. intros Hsr ? (? & ? & ? & ?)%Hsr. eexists _, _. naive_solver. Qed.
-
-  Lemma safe_reach_no_forks p e σ e' σ' (Φ : _ → _ → Prop):
-    steps_no_fork p e σ e' σ' → safe_reach p e' σ' Φ → safe_reach p e σ Φ.
-  Proof.
-    intros Hsteps Hsr Hsafe. specialize (safe_no_forks _ _ _ _ _ Hsafe Hsteps) as (?&?&?&?)%Hsr.
-    eexists _, _. split; last done. by apply: no_forks_trans.
-  Qed.
-
-  Lemma safe_reach_step p e σ e' σ' (Φ : _ → _ → Prop):
-    prim_step p e σ e' σ' [] → safe_reach p e' σ' Φ → safe_reach p e σ Φ.
-  Proof.
-    move => ??. apply: safe_reach_no_forks; [|done].
-    apply: no_forks_step; [done|]. apply: no_forks_refl.
-  Qed.
-
-  Lemma safe_reach_head_step p e σ e' σ' (Φ : _ → _ → Prop):
-    head_step p e σ e' σ' [] → safe_reach p e' σ' Φ → safe_reach p e σ Φ.
-  Proof. move => ??. apply: safe_reach_step; [|done]. by apply: head_prim_step. Qed.
-
-  Lemma fill_safe_reach p e σ Φ Ks:
-    safe_reach p e σ (post_in_ectx Φ) → safe_reach p (fill Ks e) σ (post_in_ectx Φ).
-  Proof.
-    intros Hsr (?&?&?&Hp)%fill_safe%Hsr.
-    eexists _, _. split; [ by apply: fill_no_forks | ].
-    destruct Hp as (? & ? & -> & ?).
-    eexists _, _. rewrite fill_comp. naive_solver.
-  Qed.
-
-  Lemma safe_reach_bind p e σ Φ Ks:
-    safe_reach p e σ (λ e' σ', safe_reach p (fill Ks e') σ' Φ) → safe_reach p (fill Ks e) σ Φ.
-  Proof.
-    intros Hsr Hsafe.
-    specialize (Hsr (fill_safe _ _ _ _  Hsafe)) as (? &?&?&Hp).
-    destruct Hp as (?&?& ? & ?).
-    { eapply safe_no_forks; first done. by apply fill_no_forks. }
-    eexists _, _. split; last done.
-    eapply no_forks_trans.
-    - by eapply fill_no_forks.
-    - done.
-  Qed.
-
-  Lemma pool_safe_safe_reach π p T e σ Φ K:
-    pool_safe p T σ →
-    T !! π = Some (fill K e) →
-    safe_reach p e σ Φ →
-    ∃ e' σ',  Φ e' σ' ∧ pool_safe p (<[π := fill K e']>T) σ'.
-  Proof.
-    intros Hs Hlook Hsr.
-    assert (safe p e σ) as (e' & σ' & ? & ?)%Hsr.
-    { eapply fill_safe. eapply pool_safe_threads_safe; done. }
-    eexists _, _. split; first done.
-    eapply pool_safe_no_forks; [done..|]. by apply: fill_no_forks.
-  Qed.
-
-  Lemma pool_safe_safe_reach_stuck π p T e σ Φ :
-    pool_safe p T σ →
-    T !! π = Some e →
-    safe_reach p e σ Φ →
-    (∀ e' σ', Φ e' σ' → pool_safe p (<[π := e']> T) σ' → pool_reach_stuck p (<[π := e']>T) σ') →
-    pool_reach_stuck p T σ.
-  Proof.
-    intros Hs Hlook Hsr Hp. edestruct Hsr as (e' & σ' & Hsteps & Hphi).
-    { by eapply pool_safe_threads_safe. }
-    apply Hp in Hphi.
-    - eapply pool_reach_stuck_no_forks; done.
-    - eapply pool_safe_no_forks; done.
-  Qed.
-End safe_reach.
-
-
-(* discrete OFE instance for expr and thread_id *)
+(* discrete OFE instance for expr *)
 Definition exprO {val public_state} {Λ : mlanguage val public_state} := leibnizO (expr Λ).
 Global Instance expr_equiv {val public_state} {Λ : mlanguage val public_state} : Equiv (expr Λ). apply exprO. Defined.
-
-Definition thread_idO := leibnizO thread_id.
-Global Instance thread_id_equiv : Equiv thread_id. apply thread_idO. Defined.
